

1.

$$y(x, \mathbf{w}) = w_0 + w_1x + w_2x^2 + \cdots + w_Mx^M = \sum_{j=0}^M w_j(x_n)^j$$

$$E(\mathbf{w}) = \frac{1}{2} \sum_{n=1}^N \left[y(x_n, \mathbf{w}) - t_n \right]^2$$

$$\Rightarrow E(\mathbf{w}) = \frac{1}{2} \sum_{n=1}^N \left[\sum_{j=0}^M w_j(x_n)^j - t_n \right]^2$$

$$\frac{\partial E}{\partial w_i} = \frac{1}{2} \sum_{n=1}^N 2 \left[\sum_{j=0}^M w_j(x_n)^j - t_n \right] \frac{\partial}{\partial w_i} \left[\sum_{j=0}^M w_j(x_n)^j - t_n \right]$$

$$= \sum_{n=1}^N \left[\sum_{j=0}^M w_j(x_n)^j - t_n \right] \sum_{j=0}^M (x_n)^j \frac{\partial w_i}{\partial w_j} \left(\frac{\partial w_i}{\partial w_j} = \delta_{ij} = \begin{cases} 1, & \text{if } j = i, \\ 0, & \text{if } j \neq i \end{cases} \right)$$

$$= \sum_{n=1}^N \left[\sum_{j=0}^M w_j(x_n)^j - t_n \right] (x_n)^i$$

$$\frac{\partial E}{\partial w_i} = 0$$

$$\Rightarrow \sum_{n=1}^N \left[\sum_{j=0}^M w_j(x_n)^j - t_n \right] (x_n)^i = 0$$

$$\Rightarrow \sum_{n=1}^N \sum_{j=0}^M w_j(x_n)^j (x_n)^i - \sum_{n=1}^N t_n (x_n)^i = 0$$

$$\Rightarrow \sum_{n=1}^N \sum_{j=0}^M w_j(x_n)^{j+i} - \sum_{n=1}^N t_n (x_n)^i = 0$$

$$\Rightarrow \sum_{j=0}^M w_j \sum_{n=1}^N (x_n)^{j+i} - \sum_{n=1}^N t_n (x_n)^i = 0$$

$$\Rightarrow \sum_{j=0}^M w_j \sum_{n=1}^N (x_n)^{j+i} = \sum_{n=1}^N t_n (x_n)^i$$

$$\Rightarrow \sum_{j=0}^M A_{ij} w_j = T_i \left(A_{ij} = \sum_{n=1}^N (x_n)^{j+i}, \quad T_i = \sum_{n=1}^N t_n (x_n)^i \right)$$

In matrix notation:

$$\mathbf{A} \mathbf{w} = \mathbf{T}$$

$$\Rightarrow \mathbf{w} = \mathbf{A}^{-1} \mathbf{T}$$

2.

$$y(x, \mathbf{w}) = w_0 + w_1 x + w_2 x^2 + \cdots + w_M x^M = \sum_{j=0}^M w_j (x_n)^j$$

$$\begin{aligned} \tilde{E}(\mathbf{w}) &= \frac{1}{2} \sum_{n=1}^N \left[y(x_n, \mathbf{w}) - t_n \right]^2 + \frac{\lambda}{2} \|\mathbf{w}\|^2 \\ \Rightarrow \tilde{E}(\mathbf{w}) &= \frac{1}{2} \sum_{n=1}^N \left[\sum_{j=0}^M w_j (x_n)^j - t_n \right]^2 + \frac{\lambda}{2} \sum_{j=0}^M w_j^2 \end{aligned}$$

$$\begin{aligned} \frac{\partial \tilde{E}}{\partial w_i} &= \frac{\partial}{\partial w_i} \frac{1}{2} \sum_{n=1}^N \left[\sum_{j=0}^M w_j (x_n)^j - t_n \right]^2 + \frac{\partial}{\partial w_i} \frac{\lambda}{2} \sum_{j=0}^M w_j^2 \\ &= \frac{1}{2} \sum_{n=1}^N 2 \left[\sum_{j=0}^M w_j (x_n)^j - t_n \right] \frac{\partial}{\partial w_i} \left[\sum_{j=0}^M w_j (x_n)^j - t_n \right] + \frac{\lambda}{2} \frac{\partial}{\partial w_i} \sum_{j=0}^M w_j^2 \\ &= \frac{1}{2} \sum_{n=1}^N 2 \left[\sum_{j=0}^M w_j (x_n)^j - t_n \right] \sum_{j=0}^M (x_n)^j \frac{\partial w_i}{\partial w_j} + \frac{\lambda}{2} \frac{\partial}{\partial w_i} \sum_{j=0}^M w_j^2 \left(\frac{\partial w_i}{\partial w_j} = \delta_{ij} = (x_n)^i \text{ if } j = i \right) \\ &= \sum_{n=1}^N \left[\sum_{j=0}^M w_j (x_n)^j - t_n \right] (x_n)^i + \lambda w_i \end{aligned}$$

$$\begin{aligned} \frac{\partial \tilde{E}}{\partial w_i} &= 0 \\ \Rightarrow \sum_{n=1}^N \left[\sum_{j=0}^M w_j (x_n)^j - t_n \right] (x_n)^i + \lambda w_i &= 0 \\ \Rightarrow \sum_{n=1}^N \sum_{j=0}^M w_j (x_n)^j (x_n)^i - \sum_{n=1}^N (x_n)^i t_n + \lambda w_i &= 0 \\ \Rightarrow \sum_{n=1}^N \sum_{j=0}^M w_j (x_n)^{j+i} - \sum_{n=1}^N (x_n)^i t_n + \lambda w_i &= 0 \\ \Rightarrow \sum_{j=0}^M w_j \sum_{n=1}^N (x_n)^{j+i} - \sum_{n=1}^N (x_n)^i t_n + \lambda w_i &= 0 \\ \Rightarrow \sum_{j=0}^M w_j \sum_{n=1}^N (x_n)^{j+i} + \lambda w_i = \sum_{n=1}^N (x_n)^i t_n \\ \Rightarrow \sum_{j=0}^M A_{ij} w_j + \lambda w_i = T_i \left(A_{ij} = \sum_{n=1}^N (x_n)^{j+i}, \quad T_i = \sum_{n=1}^N t_n (x_n)^i \right) \end{aligned}$$

In matrix notation:

$$\begin{aligned} \mathbf{A} \mathbf{w} + \lambda \mathbf{w} &= \mathbf{T} \\ \Rightarrow (\mathbf{A} + \lambda \mathbf{I}) \mathbf{w} &= \mathbf{T} \\ \Rightarrow \mathbf{w} &= (\mathbf{A} + \lambda \mathbf{I})^{-1} \mathbf{T} \end{aligned}$$

4.

$$E[L(\mathbf{t}, \mathbf{y}(x))] = \int \int \|\mathbf{y}(x) - \mathbf{t}\|^2 p(x, t) dx dt.$$

Often, this is simply written as: $E[L] = \int \int \|\mathbf{y}(x) - \mathbf{t}\|^2 p(x, t) dx dt.$

Since $\|\mathbf{y}(x) - \mathbf{t}\|^2 = (\mathbf{y}(x) - \mathbf{t})^\top (\mathbf{y}(x) - \mathbf{t})$,

we can expand it as: $\|\mathbf{y}(x) - \mathbf{t}\|^2 = \sum_{i=1}^M [\mathbf{y}_i(x) - \mathbf{t}_i]^2.$

Hence: $E[L] = \int \int \sum_{i=1}^M [\mathbf{y}_i(x) - \mathbf{t}_i]^2 p(x, t) dx dt.$

$$\begin{aligned} \delta E[L] &= \frac{\delta}{\delta \mathbf{y}_j(x)} \int \int \sum_{i=1}^M [\mathbf{y}_i(x) - \mathbf{t}_i]^2 p(x, t) dx dt \\ &= \int \int \frac{\delta}{\delta \mathbf{y}_j(x)} \left[\sum_{i=1}^M (\mathbf{y}_i(x) - \mathbf{t}_i)^2 \right] p(x, t) dx dt. \end{aligned}$$

Inside the summation, the only term that depends on $\mathbf{y}_j(x)$ is $(\mathbf{y}_j(x) - \mathbf{t}_j)^2$. Its derivative is:

$$\frac{\delta}{\delta \mathbf{y}_j(x)} \left[(\mathbf{y}_j(x) - \mathbf{t}_j)^2 \right] = 2[\mathbf{y}_j(x) - \mathbf{t}_j].$$

Thus:

$$\frac{\delta}{\delta \mathbf{y}_j(x)} \left[\sum_{i=1}^M (\mathbf{y}_i(x) - \mathbf{t}_i)^2 \right] = 2[\mathbf{y}_j(x) - \mathbf{t}_j].$$

Substituting this back, we have:

$$\frac{\delta E[L]}{\delta \mathbf{y}_j(x)} = \int \int 2[\mathbf{y}_j(x) - \mathbf{t}_j] p(x, t) dx dt.$$

$$\frac{\delta E[L]}{\delta \mathbf{y}_j(x)} = 2 \int [\mathbf{y}_j(x) - \mathbf{t}_j] p(t | x) dt,$$

where $p(t | x) = \frac{p(x, t)}{p(x)}$.

$$\frac{\delta E[L]}{\delta \mathbf{y}_j(x)} = 0 \implies \int 2[\mathbf{y}_j(x) - \mathbf{t}_j] p(x, t) dt = 0.$$

Divide out the constant 2:

$$\int [\mathbf{y}_j(x) - \mathbf{t}_j] p(x, t) dt = 0.$$

Distribute inside the integral:

$$\mathbf{y}_j(x) \int p(x, t) dt - \int \mathbf{t}_j p(x, t) dt = 0.$$

Since $\int p(x, t) dt = p(x)$, we get:

$$\mathbf{y}_j(x)p(x) = \int \mathbf{t}_j p(x, t) dt.$$

$$\mathbf{y}(x) = \frac{\int \mathbf{t} p(t, x) dt}{\int p(t, x) dt} = \int \mathbf{t} p(t | x) dt.$$

$$\mathbf{y}_j(x) = \frac{\int \mathbf{t}_j p(x, t) dt}{\int p(x, t) dt} = \frac{\int \mathbf{t}_j p(x, t) dt}{p(x)} = \mathbb{E}[\mathbf{t}_j | x].$$

5.

$$\text{Bin}(m | N, \mu) = \binom{N}{m} \mu^m (1 - \mu)^{N-m}$$

$$\binom{N}{m} + \binom{N}{m-1} = \binom{N+1}{m}$$

$$\binom{N}{m} = \frac{N!}{m! (N-m)!}$$

$$\binom{N}{m-1} = \frac{N!}{(m-1)! [N - (m-1)]!} = \frac{N!}{(m-1)! (N-m+1)!}$$

$$\begin{aligned} \binom{N}{m} + \binom{N}{m-1} &= \frac{N!}{m!(N-m)!} + \frac{N!}{(m-1)!(N-m+1)!} \\ &= \frac{N!}{m(m-1)!(N-m)!} + \frac{N!}{(m-1)!(N-m+1)(N-m)!} \\ &\quad (\text{As } m! = m(m-1)! \text{ and } (N-m+1)! = (N-m+1)(N-m)!) \\ &= \frac{N!}{(N-m)!(m-1)!} \frac{1}{m} + \frac{N!}{(N-m)!(m-1)!} \frac{1}{N-m+1} \\ &= \frac{N!}{(N-m)!(m-1)!} \left(\frac{1}{m} + \frac{1}{N-m+1} \right) \\ &= \frac{N!}{(N-m)!(m-1)!} \left(\frac{N-m+1+m}{m(N-m+1)} \right) \\ &= \frac{N!}{(N-m)!(m-1)!} \left(\frac{N+1}{m(N-m+1)} \right). \end{aligned}$$

$$\begin{aligned} \binom{N+1}{m} &= \frac{(N+1)!}{m! [(N+1)-m]!} = \frac{(N+1)!}{m! (N+1-m)!} \\ &= \frac{(N+1) N!}{m(m-1)!(N+1-m)(N-m)!} \\ &= \frac{N!}{(N-m)!(m-1)!} \frac{N+1}{m(N+1-m)}. \end{aligned}$$

Since the expressions for $\binom{N}{m} + \binom{N}{m-1}$ and $\binom{N+1}{m}$ match, identity is proven:

$$\binom{N}{m} + \binom{N}{m-1} = \binom{N+1}{m}.$$

$$(1+x)^N = \sum_{m=0}^N \binom{N}{m} x^m, \quad \text{where } \binom{N}{m} = \frac{N!}{m!(N-m)!}.$$

Base Case: $N = 0$

When $N = 0$, the left-hand side is

$$(1+x)^0 = 1.$$

The right-hand side is

$$\sum_{m=0}^0 \binom{0}{m} x^m = \binom{0}{0} x^0 = 1,$$

because $\binom{0}{0} = 1$ and $x^0 = 1$.

Inductive Step: From N to $N+1$

Start with the left-hand side at $N+1$:

$$(1+x)^{N+1} = (1+x)(1+x)^N.$$

By the inductive hypothesis, we know that $(1+x)^N$ is

$$\sum_{m=0}^N \binom{N}{m} x^m.$$

Substitute this into the equation:

$$(1+x)^{N+1} = (1+x) \sum_{m=0}^N \binom{N}{m} x^m.$$

$$(1+x)^{N+1} = \sum_{m=0}^N \binom{N}{m} x^m + \sum_{m=0}^N \binom{N}{m} x^{m+1}$$

$$(1+x)^{N+1} = \binom{N}{0} x^0 + \sum_{m=1}^N \binom{N}{m} x^m + \sum_{m=1}^{N+1} \binom{N}{m-1} x^m$$

At $m = 0$, we only have

$$\binom{N}{0} x^0 = 1.$$

At $m = N+1$, we only have

$$\binom{N}{(N+1)-1} x^{N+1} = \binom{N}{N} x^{N+1} = x^{N+1}.$$

$$(1+x)^{N+1} = \binom{N}{0} x^0 + \sum_{m=1}^N \left[\binom{N}{m} + \binom{N}{m-1} \right] x^m + \binom{N}{N} x^{N+1} \quad (1)$$

Use this to simplify each bracketed pair:

$$\binom{N}{m} + \binom{N}{m-1} = \binom{N+1}{m}.$$

Thus, for $1 \leq m \leq N$, each pair becomes

$$\binom{N+1}{m} x^m.$$

Also note:

$$\binom{N}{0} = 1, \quad \binom{N+1}{0} = 1, \quad \binom{N}{N} = 1, \quad \binom{N+1}{N+1} = 1.$$

Hence, the expression reorganizes as:

$$(1+x)^{N+1} = \binom{N+1}{0} x^0 + \sum_{m=1}^N \binom{N+1}{m} x^m + \binom{N+1}{N+1} x^{N+1}.$$

But this is simply the sum from $m = 0$ to $m = N + 1$:

$$(1+x)^{N+1} = \sum_{m=0}^{N+1} \binom{N+1}{m} x^m.$$

Base Case: $N = 0$: Verified

$$(1+x)^0 = 1.$$

Inductive Step: Shown that if

$$(1+x)^N = \sum_{m=0}^N \binom{N}{m} x^m,$$

then

$$(1+x)^{N+1} = \sum_{m=0}^{N+1} \binom{N+1}{m} x^m.$$

By the Principle of Mathematical Induction, we have proved that, for all integers $N \geq 0$,

$$(1+x)^N = \sum_{m=0}^N \binom{N}{m} x^m.$$

Binomial Distribution:

$$\text{Bin}(m \mid N, \mu) = \binom{N}{m} \mu^m (1-\mu)^{N-m}, \quad m = 0, 1, \dots, N.$$

We want to show that this distribution sums to 1:

$$\sum_{m=0}^N \binom{N}{m} \mu^m (1-\mu)^{N-m} = 1.$$

2. Binomial Theorem:

From the binomial theorem, we know:

$$(1+x)^N = \sum_{m=0}^N \binom{N}{m} x^m \quad \text{for any real (or complex) } x.$$

3. Applying the Theorem to the Binomial Distribution:

Choose $x = \frac{\mu}{1-\mu}$. However, an even simpler approach is to directly observe that:

$$\mu + (1-\mu) = 1.$$

Hence, if we set $\alpha = \mu$ and $\beta = 1 - \mu$ in the binomial theorem, we get:

$$(\alpha + \beta)^N = \sum_{m=0}^N \binom{N}{m} \alpha^m \beta^{N-m}.$$

Then $\alpha + \beta = \mu + (1 - \mu) = 1$, so the left-hand side is:

$$1^N = 1.$$

Meanwhile, the right-hand side is:

$$\sum_{m=0}^N \binom{N}{m} \mu^m (1 - \mu)^{N-m}.$$

Putting it together:

$$1 = \sum_{m=0}^N \binom{N}{m} \mu^m (1 - \mu)^{N-m}.$$

4. Conclusion:

Thus, we have shown that:

$$\sum_{m=0}^N \text{Bin}(m \mid N, \mu) = \sum_{m=0}^N \binom{N}{m} \mu^m (1 - \mu)^{N-m} = 1,$$

demonstrating that the binomial distribution is properly normalized.